{-# OPTIONS --without-K --safe #-}

open import Axiom.Extensionality.Propositional

-- Cumulativity of the gluing models for terms and types
module Mints.Soundness.Cumulativity (fext : ∀ {ℓ ℓ′} → Extensionality ℓ ℓ′) where

open import Lib
open import Data.Nat.Properties as ℕₚ

open import Mints.Statics.Properties
open import Mints.Semantics.Readback
open import Mints.Semantics.Properties.PER fext
open import Mints.Soundness.LogRel
open import Mints.Soundness.Realizability fext
open import Mints.Soundness.Properties.LogRel fext


-- Similar to cumulativity of the PER model, we also need a lowering lemma in order to
-- establish cumulativity (®El-lower).  Unlike the PER model, lowering in the gluing
-- model is a bit more difficult because we need to have one extra assumption of
-- syntactic and semantic types glued in the lower level. By exploiting this
-- assumption, we replace everything about types to the lower level in the gluing of
-- terms.
mutual

  ®-cumu-step : ∀ {i} (A≈B : A ≈ B ∈ 𝕌 i) →
                Γ ⊢ T ®[ i ] A≈B →
                -----------------------------
                Γ ⊢ T ®[ suc i ] 𝕌-cumu-step i A≈B
  ®-cumu-step (ne C≈C′) (⊢T , rel) = cumu ⊢T , λ ⊢σ → ≈-cumu (rel ⊢σ)
  ®-cumu-step N T∼A                = ≈-cumu T∼A
  ®-cumu-step (U′ j<i) T∼A         = ≈-cumu T∼A
  ®-cumu-step (□ A≈B) T∼A          = record
    { GT   = GT
    ; T≈   = ≈-cumu T≈
    ; krip = λ {_} {σ} Ψs ⊢ΨsΔ ⊢σ → ®-cumu-step (A≈B (ins (mt σ) (len Ψs))) (krip Ψs ⊢ΨsΔ ⊢σ)
    }
    where open Glu□ T∼A
  ®-cumu-step (Π iA RT) T∼A        = record
    { IT   = IT
    ; OT   = OT
    ; ⊢OT  = cumu ⊢OT
    ; T≈   = ≈-cumu T≈
    ; krip = λ {_} {σ} ⊢σ →
      let open ΠRel (krip ⊢σ)
      in record
      { IT-rel = ®-cumu-step (iA (mt σ)) IT-rel
      ; OT-rel = λ s∼a a∈ → ®-cumu-step (ΠRT.T≈T′ (RT (mt σ) (El-lower _ (iA (mt σ)) a∈))) (OT-rel (®El-lower (iA (mt σ)) IT-rel s∼a) (El-lower _ (iA (mt σ)) a∈))
      }
    }
    where open GluΠ T∼A


  ®El-cumu-step : ∀ {i} (A≈B : A ≈ B ∈ 𝕌 i) →
                  Γ ⊢ t ∶ T ®[ i ] a ∈El A≈B →
                  ------------------------------------------
                  Γ ⊢ t ∶ T ®[ suc i ] a ∈El 𝕌-cumu-step i A≈B
  ®El-cumu-step (ne C≈C′) (ne c∈ , rel)    = ne c∈ , record
    { t∶T  = t∶T
    ; ⊢T   = cumu ⊢T
    ; krip = λ ⊢σ → let Tσ≈ , tσ≈ = krip ⊢σ in ≈-cumu Tσ≈ , tσ≈
    }
    where open GluNe rel
  ®El-cumu-step N (t∼a , T≈N)              = t∼a , ≈-cumu T≈N
  ®El-cumu-step (U′ j<i) t∼a
    rewrite Glu-wellfounded-≡ j<i
          | Glu-wellfounded-≡ (≤-step j<i) = record
    { t∶T = t∶T
    ; T≈  = ≈-cumu T≈
    ; A∈𝕌 = A∈𝕌
    ; rel = rel
    }
    where open GluU t∼a
  ®El-cumu-step (□ A≈B) t∼a                = record
    { GT   = GT
    ; t∶T  = t∶T
    ; a∈El = El-cumu-step _ (□ A≈B) a∈El
    ; T≈   = ≈-cumu T≈
    ; krip = λ {_} {σ} Ψs ⊢ΨsΔ ⊢σ →
      let open □Krip (krip Ψs ⊢ΨsΔ ⊢σ)
      in record
      { ua  = ua
      ; ↘ua = ↘ua
      ; rel = ®El-cumu-step (A≈B (ins (mt σ) (len Ψs))) rel
      }
    }
    where open Glubox t∼a
  ®El-cumu-step (Π iA RT) t∼a              = record
    { t∶T  = t∶T
    ; a∈El = El-cumu-step _ (Π iA RT) a∈El
    ; IT   = IT
    ; OT   = OT
    ; ⊢OT  = cumu ⊢OT
    ; T≈   = ≈-cumu T≈
    ; krip = λ {_} {σ} ⊢σ →
      let open ΛRel (krip ⊢σ)
      in record
      { IT-rel = ®-cumu-step (iA (mt σ)) IT-rel
      ; ap-rel = λ s∼b b∈ →
        let open ΛKripke (ap-rel (®El-lower (iA (mt σ)) IT-rel s∼b) (El-lower _ (iA (mt σ)) b∈))
        in record
        { fa  = fa
        ; ↘fa = ↘fa
        ; ®fa = ®El-cumu-step (ΠRT.T≈T′ (RT (mt σ) (El-lower _ (iA (mt σ)) b∈))) ®fa
        }
      }
    }
    where open GluΛ t∼a


  -- This is tricky! We need to pass on the knowledge that T is related to A in a
  -- lower level such that ®El can be lowered! It cannot be done without this extra
  -- piece of knowledge.
  ®El-lower : ∀ {i} (A≈B : A ≈ B ∈ 𝕌 i) →
              Γ ⊢ T ®[ i ] A≈B →  --  This assumption is critically needed.
              Γ ⊢ t ∶ T ®[ suc i ] a ∈El 𝕌-cumu-step i A≈B →
              -----------------------------------------
              Γ ⊢ t ∶ T ®[ i ] a ∈El A≈B
  ®El-lower (ne C≈C′) (⊢T , rel) (ne c∈⊥ , rel′) = ne c∈⊥ , record
    { t∶T  = t∶T
    ; ⊢T   = ⊢T
    ; krip = λ ⊢σ → rel ⊢σ , proj₂ (krip ⊢σ)
    }
    where open GluNe rel′ hiding (⊢T)
  ®El-lower N T∼A (t∼a , _)                      = t∼a , T∼A
  ®El-lower (U′ j<i) T∼A t∼a
    rewrite Glu-wellfounded-≡ j<i
          | Glu-wellfounded-≡ (≤-step j<i)       = record
    { t∶T = t∶T
    ; T≈  = T∼A
    ; A∈𝕌 = A∈𝕌
    ; rel = rel
    }
    where open GluU t∼a
  ®El-lower (□ A≈B) T∼A t∼a                      = record
    { GT   = T.GT
    ; t∶T  = t∶T
    ; a∈El = El-lower _ (□ A≈B) a∈El
    ; T≈   = T.T≈
    ; krip = λ {_} {σ} Ψs ⊢ΨsΔ ⊢σ →
      let open □Krip (krip Ψs ⊢ΨsΔ ⊢σ)
          A≈Bcu = A≈B (ins (mt σ) (len Ψs))
      in record
      { ua  = ua
      ; ↘ua = ↘ua
      ; rel = ®El-lower (A≈B (ins (mt σ) (len Ψs)))
                        (T.krip Ψs ⊢ΨsΔ ⊢σ)
                        (®El-resp-T≈ (𝕌-cumu-step _ (A≈B (ins (mt σ) (len Ψs))))
                                     rel
                                     (≈-sym (®⇒≈ (𝕌-cumu-step _ A≈Bcu) (®-cumu-step A≈Bcu (T.krip Ψs ⊢ΨsΔ ⊢σ)) (®El⇒® (𝕌-cumu-step _ A≈Bcu) rel))))
      }
    }
    where module T = Glu□ T∼A
          open Glubox t∼a
  ®El-lower (Π iA RT) T∼A t∼a                    = record
    { t∶T  = t∶T
    ; a∈El = El-lower _ (Π iA RT) a∈El
    ; IT   = T.IT
    ; OT   = T.OT
    ; ⊢OT  = T.⊢OT
    ; T≈   = T.T≈
    ; krip = λ {_} {σ} ⊢σ →
      let open ΛRel (krip ⊢σ)
          module Π = ΠRel (T.krip ⊢σ)
          iAcu = 𝕌-cumu-step _ (iA (mt σ))
      in record
      { IT-rel = Π.IT-rel
      ; ap-rel = λ s∼b b∈ →
        let open ΛKripke (ap-rel (®El-resp-T≈ iAcu
                                              (®El-cumu-step (iA (mt σ)) s∼b)
                                              (®⇒≈ iAcu (®-cumu-step (iA (mt σ)) Π.IT-rel) IT-rel))
                                 (El-cumu-step _ (iA (mt σ)) b∈))
            RT₁      = RT (mt σ) b∈
            RT₂      = RT (mt σ) (El-lower _ (iA (mt σ)) (El-cumu-step _ (iA (mt σ)) b∈))
            T≈T′     = ΠRT.T≈T′ RT₁
            T≈T′cumu = 𝕌-cumu-step _ T≈T′
            ®fa′     = ®El-≡ (𝕌-cumu-step _ (ΠRT.T≈T′ RT₂))
                             T≈T′cumu
                             ®fa
                             (⟦⟧-det (ΠRT.↘⟦T⟧ RT₂) (ΠRT.↘⟦T⟧ RT₁))
        in record
        { fa  = fa
        ; ↘fa = ↘fa
        ; ®fa = ®El-lower T≈T′ (Π.OT-rel s∼b b∈)
                          (®El-resp-T≈ T≈T′cumu ®fa′
                                       (®⇒≈ T≈T′cumu (®El⇒® T≈T′cumu ®fa′) (®-cumu-step T≈T′ (Π.OT-rel s∼b b∈))))
        }
      }
    }
    where module T = GluΠ T∼A
          open GluΛ t∼a

-- Push cumulativity to any higher level.
®-cumu-steps : ∀ {i} j
               (A≈B : A ≈ B ∈ 𝕌 i) →
               Γ ⊢ T ®[ i ] A≈B →
               -----------------------------
               Γ ⊢ T ®[ j + i ] 𝕌-cumu-steps i j A≈B
®-cumu-steps zero A≈B T∼A    = T∼A
®-cumu-steps (suc j) A≈B T∼A = ®-cumu-step (𝕌-cumu-steps _ j A≈B) (®-cumu-steps j A≈B T∼A)


®El-cumu-steps : ∀ {i} j
                 (A≈B : A ≈ B ∈ 𝕌 i) →
                 Γ ⊢ t ∶ T ®[ i ] a ∈El A≈B →
                 ------------------------------------------
                 Γ ⊢ t ∶ T ®[ j + i ] a ∈El 𝕌-cumu-steps i j A≈B
®El-cumu-steps zero A≈B t∼a    = t∼a
®El-cumu-steps (suc j) A≈B t∼a = ®El-cumu-step (𝕌-cumu-steps _ j A≈B) (®El-cumu-steps j A≈B t∼a)


®-cumu : ∀ {i j}
         (A≈B : A ≈ B ∈ 𝕌 i) →
         Γ ⊢ T ®[ i ] A≈B →
         (i≤j : i ≤ j) →
         -----------------------------
         Γ ⊢ T ®[ j ] 𝕌-cumu i≤j A≈B
®-cumu {i = i} A≈B T∼A i≤j
  with ®-cumu-steps (≤-diff i≤j) A≈B T∼A
...  | rel = helper (𝕌-cumu-steps i (≤-diff i≤j) A≈B) (𝕌-cumu i≤j A≈B) rel (trans (ℕₚ.+-comm (≤-diff i≤j) i) (≤-diff-+ i≤j))
  where helper : ∀ {i j} (A≈B : A ≈ B ∈ 𝕌 i) (A≈B′ : A ≈ B ∈ 𝕌 j) → Γ ⊢ T ®[ i ] A≈B → i ≡ j → Γ ⊢ T ®[ j ] A≈B′
        helper A≈B A≈B′ T∼A refl = ®-one-sided A≈B A≈B′ T∼A

®El-cumu : ∀ {i j}
           (A≈B : A ≈ B ∈ 𝕌 i) →
           Γ ⊢ t ∶ T ®[ i ] a ∈El A≈B →
           (i≤j : i ≤ j) →
           -----------------------------
           Γ ⊢ t ∶ T ®[ j ] a ∈El 𝕌-cumu i≤j A≈B
®El-cumu {i = i} A≈B t∼a i≤j
  with ®El-cumu-steps (≤-diff i≤j) A≈B t∼a
...  | rel = helper (𝕌-cumu-steps i (≤-diff i≤j) A≈B) (𝕌-cumu i≤j A≈B) rel (trans (ℕₚ.+-comm (≤-diff i≤j) i) (≤-diff-+ i≤j))
  where helper : ∀ {i j} (A≈B : A ≈ B ∈ 𝕌 i) (A≈B′ : A ≈ B ∈ 𝕌 j) → Γ ⊢ t ∶ T ®[ i ] a ∈El A≈B → i ≡ j → Γ ⊢ t ∶ T ®[ j ] a ∈El A≈B′
        helper A≈B A≈B′ t∼a refl = ®El-one-sided A≈B A≈B′ t∼a

®El-lowers : ∀ {i} j
             (A≈B : A ≈ B ∈ 𝕌 i) →
             Γ ⊢ T ®[ i ] A≈B →
             Γ ⊢ t ∶ T ®[ j + i ] a ∈El 𝕌-cumu-steps i j A≈B →
             -----------------------------
             Γ ⊢ t ∶ T ®[ i ] a ∈El A≈B
®El-lowers 0       A≈B T∼A t∼a = t∼a
®El-lowers (suc j) A≈B T∼A t∼a = ®El-lowers j A≈B T∼A (®El-lower (𝕌-cumu-steps _ j A≈B) (®-cumu-steps j A≈B T∼A) t∼a)


-- Given cumulativity and lowering, we can obtain a generalization of both, stating
-- that if types are related in any level, then we can adjust the gluing for terms to
-- this level, regardless of the original level.
®El-irrel : ∀ {i j}
            (A≈B : A ≈ B ∈ 𝕌 i) →
            (A≈B′ : A ≈ B′ ∈ 𝕌 j) →
            Γ ⊢ T ®[ j ] A≈B′ →
            Γ ⊢ t ∶ T ®[ i ] a ∈El A≈B →
            -----------------------------
            Γ ⊢ t ∶ T ®[ j ] a ∈El A≈B′
®El-irrel {i = i} {j} A≈B A≈B′ T∼A t∼a
  with i ≤? j
...  | yes i≤j = ®El-one-sided (𝕌-cumu i≤j A≈B) A≈B′ (®El-cumu A≈B t∼a i≤j)
...  | no  i≰j
    with ≰⇒≥ i≰j
...    | i≥j
      rewrite sym (m∸n+n≡m i≥j) = ®El-lowers (i ∸ j) A≈B′ T∼A (®El-one-sided A≈B (𝕌-cumu-steps _ (i ∸ j) A≈B′) t∼a)


-- The master lemma which handles everything you need to deal with universe levels.
--
-- This proof is not very straightforward. We have:
--
--     A ≈ A′ at level i
--     B ≈ B′ at level j
--     A ≈ B at level k
--     t : T ∼ a ∈ El A at level i
--     T ≈ T′ at level k
--
-- Our goal is t : T′ ∼ a ∈ El B at level j
--
-- We proceed as follows:
--
-- t : T  ∼ a ∈ El A at level max i k          (by cumulativity)
-- t : T′ ∼ a ∈ El A at level max i k          (T ≈ T′ at level max i k)
-- t : T′ ∼ a ∈ El A at level max j (max i k)  (cumulativity)
--
-- The previous step lifts the gluing relation to a high enough level so that we can
-- move a to B
--
-- t : T′ ∼ a ∈ El B at level max j (max i k)  (by transportation due to A ≈ B)
-- t : T′ ∼ a ∈ El B at level j                (by lowering)
®El-master : ∀ {i j k} →
             (A≈A′ : A ≈ A′ ∈ 𝕌 i)
             (B≈B′ : B ≈ B′ ∈ 𝕌 j)
             (A≈B : A ≈ B ∈ 𝕌 k) →
             Γ ⊢ T′ ®[ j ] B≈B′ →
             Γ ⊢ t ∶ T ®[ i ] a ∈El A≈A′ →
             Γ ⊢ T ≈ T′ ∶ Se k →
             ------------------------------
             Γ ⊢ t ∶ T′ ®[ j ] a ∈El B≈B′
®El-master {i = i} {j} {k} A≈A′ B≈B′ A≈B T′∼B t∼a T≈T′
  = ®El-irrel B≈B′↑ B≈B′ T′∼B
    (®El-transport A≈A′↑↑ B≈B′↑ (𝕌-cumu k≤m′ A≈B)
    (®El-cumu A≈A′↑
    (®El-resp-T≈ A≈A′↑
    (®El-cumu A≈A′ t∼a i≤m) (lift-⊢≈-Se-max′ T≈T′))
              m≤m′))
  where m      = max i k
        i≤m    = m≤m⊔n i k
        k≤m    = m≤n⊔m i k
        m′     = max j m
        j≤m′   = m≤m⊔n j m
        m≤m′   = m≤n⊔m j m
        k≤m′   = ≤-trans k≤m m≤m′
        A≈A′↑  = 𝕌-cumu i≤m A≈A′
        A≈A′↑↑ = 𝕌-cumu m≤m′ A≈A′↑
        B≈B′↑  = 𝕌-cumu j≤m′ B≈B′
