{-# OPTIONS --without-K --safe #-}

open import Axiom.Extensionality.Propositional

-- Proof of the fundamental theorem of soundness
module Mints.Soundness.Fundamental (fext : ∀ {ℓ ℓ′} → Extensionality ℓ ℓ′) where

open import Lib
open import Data.Nat.Properties as ℕₚ

open import Mints.Statics.Properties
open import Mints.Soundness.LogRel
open import Mints.Soundness.Typing as S hiding (⊢_; _⊢_∶_; _⊢s_∶_)
open import Mints.Soundness.Equiv
open import Mints.Soundness.Contexts fext
open import Mints.Soundness.Box fext
open import Mints.Soundness.Nat fext
open import Mints.Soundness.Pi fext
open import Mints.Soundness.Substitutions fext
open import Mints.Soundness.Terms fext
open import Mints.Soundness.Universe fext

mutual
  fundamental-⊢⇒⊩′ : S.⊢ Γ →
                     -------
                     ⊩ Γ
  fundamental-⊢⇒⊩′ ⊢[]        = ⊢[]′
  fundamental-⊢⇒⊩′ (⊢κ ⊢Γ)    = ⊢κ′ (fundamental-⊢⇒⊩′ ⊢Γ)
  fundamental-⊢⇒⊩′ (⊢∺ ⊢Γ ⊢T) = ⊢∺′ (fundamental-⊢t⇒⊩t′ ⊢T)

  fundamental-⊢t⇒⊩t′ : Γ S.⊢ t ∶ T →
                       -------------
                       Γ ⊩ t ∶ T
  fundamental-⊢t⇒⊩t′ (N-wf i ⊢Γ)            = N-wf′ i (fundamental-⊢⇒⊩′ ⊢Γ)
  fundamental-⊢t⇒⊩t′ (Se-wf i ⊢Γ)           = Se-wf′ (fundamental-⊢⇒⊩′ ⊢Γ)
  fundamental-⊢t⇒⊩t′ (Π-wf ⊢S ⊢T)           = Π-wf′ (fundamental-⊢t⇒⊩t′ ⊢S) (fundamental-⊢t⇒⊩t′ ⊢T)
  fundamental-⊢t⇒⊩t′ (□-wf ⊢T)              = □-wf′ (fundamental-⊢t⇒⊩t′ ⊢T)
  fundamental-⊢t⇒⊩t′ (vlookup ⊢Γ x∈)        = vlookup′ (fundamental-⊢⇒⊩′ ⊢Γ) x∈
  fundamental-⊢t⇒⊩t′ (ze-I ⊢Γ)              = ze-I′ (fundamental-⊢⇒⊩′ ⊢Γ)
  fundamental-⊢t⇒⊩t′ (su-I ⊢t)              = su-I′ (fundamental-⊢t⇒⊩t′ ⊢t)
  fundamental-⊢t⇒⊩t′ (N-E ⊢T ⊢s ⊢r ⊢t)      = N-E′ (fundamental-⊢t⇒⊩t′ ⊢T) (fundamental-⊢t⇒⊩t′ ⊢s) (fundamental-⊢t⇒⊩t′ ⊢r) (fundamental-⊢t⇒⊩t′ ⊢t)
  fundamental-⊢t⇒⊩t′ (Λ-I ⊢t)               = Λ-I′ (fundamental-⊢t⇒⊩t′ ⊢t)
  fundamental-⊢t⇒⊩t′ (Λ-E ⊢T ⊢r ⊢s)         = Λ-E′ (fundamental-⊢t⇒⊩t′ ⊢T) (fundamental-⊢t⇒⊩t′ ⊢r) (fundamental-⊢t⇒⊩t′ ⊢s)
  fundamental-⊢t⇒⊩t′ (□-I ⊢t)               = □-I′ (fundamental-⊢t⇒⊩t′ ⊢t)
  fundamental-⊢t⇒⊩t′ (□-E Ψs ⊢T ⊢t ⊢ΨsΓ eq) = □-E′ Ψs (fundamental-⊢t⇒⊩t′ ⊢T) (fundamental-⊢t⇒⊩t′ ⊢t) (fundamental-⊢⇒⊩′ ⊢ΨsΓ) eq
  fundamental-⊢t⇒⊩t′ (t[σ] ⊢t ⊢σ)           = t[σ]′ (fundamental-⊢t⇒⊩t′ ⊢t) (fundamental-⊢s⇒⊩s′ ⊢σ)
  fundamental-⊢t⇒⊩t′ (cumu ⊢t)              = cumu′ (fundamental-⊢t⇒⊩t′ ⊢t)
  fundamental-⊢t⇒⊩t′ (conv ⊢t T′≈T)         = conv′ (fundamental-⊢t⇒⊩t′ ⊢t) T′≈T

  fundamental-⊢s⇒⊩s′ : Γ S.⊢s σ ∶ Δ →
                       ---------------
                       Γ ⊩s σ ∶ Δ
  fundamental-⊢s⇒⊩s′ (s-I ⊢Γ)             = s-I′ (fundamental-⊢⇒⊩′ ⊢Γ)
  fundamental-⊢s⇒⊩s′ (s-wk ⊢Γ)            = s-wk′ (fundamental-⊢⇒⊩′ ⊢Γ)
  fundamental-⊢s⇒⊩s′ (s-∘ ⊢τ ⊢σ)          = s-∘′ (fundamental-⊢s⇒⊩s′ ⊢τ) (fundamental-⊢s⇒⊩s′ ⊢σ)
  fundamental-⊢s⇒⊩s′ (s-, ⊢σ ⊢T ⊢t)       = s-,′ (fundamental-⊢s⇒⊩s′ ⊢σ) (fundamental-⊢t⇒⊩t′ ⊢T) (fundamental-⊢t⇒⊩t′ ⊢t)
  fundamental-⊢s⇒⊩s′ (s-； Ψs ⊢σ ⊢ΨsΓ eq) = s-；′ Ψs (fundamental-⊢s⇒⊩s′ ⊢σ) (fundamental-⊢⇒⊩′ ⊢ΨsΓ) eq
  fundamental-⊢s⇒⊩s′ (s-conv ⊢σ Δ′≈Δ)     = s-conv′ (fundamental-⊢s⇒⊩s′ ⊢σ) Δ′≈Δ


fundamental-⊢⇒⊩ : ⊢ Γ →
                  -------
                  ⊩ Γ
fundamental-⊢⇒⊩ ⊢Γ = fundamental-⊢⇒⊩′ (C⇒S-⊢ ⊢Γ)


fundamental-⊢t⇒⊩t : Γ ⊢ t ∶ T →
                    -------------
                    Γ ⊩ t ∶ T
fundamental-⊢t⇒⊩t ⊢t = fundamental-⊢t⇒⊩t′ (C⇒S-tm ⊢t)


fundamental-⊢s⇒⊩s : Γ ⊢s σ ∶ Δ →
                    ---------------
                    Γ ⊩s σ ∶ Δ
fundamental-⊢s⇒⊩s ⊢σ = fundamental-⊢s⇒⊩s′ (C⇒S-s ⊢σ)
